# Expression Evaluation

**Expression 1:** `!A && B`
<br>
**Expression 2:** `B && !A`

These two expressions are the same. 
<br>
Here is the truth table:

| A | B | !A | !A && B | B && !A |
|---|---|----|---------|---------| 
| 0 | 0 | 1 | 0 | 0 |
| 0 | 1 | 1 | 1 | 1 |
| 1 | 0 | 0 | 0 | 0 |
| 1 | 1 | 0 | 0 | 0 |

**Expression 1:** `!A || B`
<br>
**Expression 2:** `B || !A`

These two expressions are not the same. 
<br>
Here is the truth table:

| A | B | !A | !A \|\| B | B \|\| !A |
|---|---|----|---------|---------| 
| 0 | 0 | 1 | 1 | 1 |
| 0 | 1 | 1 | 1 | 1 |
| 1 | 0 | 0 | 0 | 0 |
| 1 | 1 | 0 | 1 | 1 |

**Expression 1:** `!(A && B)`
<br>
**Expression 2:** `A || B`

These two expressions are not the same. 
<br>
Here is the truth table:

| A | B | A && B | !(A && B) | A \|\| B |
|---|---|--------|------------|---------| 
| 0 | 0 | 0 | 1 | 0 |
| 0 | 1 | 0 | 1 | 1 |
| 1 | 0 | 0 | 1 | 1 |
| 1 | 1 | 1 | 0 | 1 |

**Expression 1:** `A && B || C `
<br>
**Expression 2:**  `A && (B || C)`

These two expressions are not the same. 
<br>
Here is the truth table:

| A | B | C | A && B | `A && B \|\| C` | B \|\| C | `A && (B \|\| C)` |
|---|---|---|--------|------------|---|---------| 
| 0 | 0 | 0 | 0 | 0 | 0 | 0 |
| 0 | 0 | 1 | 0 | 1 | 1 | 0 |
| 0 | 1 | 0 | 0 | 0 | 1 | 0 |
| 0 | 1 | 1 | 0 | 1 | 1 | 0 |
| 1 | 0 | 0 | 0 | 0 | 0 | 0 |
| 1 | 0 | 1 | 0 | 1 | 1 | 1 |
| 1 | 1 | 0 | 1 | 1 | 1 | 1 |
| 1 | 1 | 1 | 1 | 1 | 1 | 1 |

**Expression 1:** `(A && B || C) `
<br>
**Expression 2:**  `!(A || B && C))`

These two expressions are not the same. 
<br>
Here is the truth table:

| A | B | C | A && B | `A && B \|\| C` | B && C | A \|\| B && C | `!(A \|\| B && C)`
|---|---|---|--------|------------|---|---------| ---------| 
| 0 | 0 | 0 | 0 | 0 | 0 | 0 | 1
| 0 | 0 | 1 | 0 | 1 | 0 | 0 | 1
| 0 | 1 | 0 | 0 | 0 | 0 | 0 | 1
| 0 | 1 | 1 | 0 | 1 | 1 | 0 | 1
| 1 | 0 | 0 | 0 | 0 | 0 | 1 | 0
| 1 | 0 | 1 | 0 | 1 | 0 | 1 | 0
| 1 | 1 | 0 | 1 | 1 | 0 | 1 | 0
| 1 | 1 | 1 | 1 | 1 | 1 | 1 | 0
 
## Complex Expressions

### Expression 1 vs Expression 2

**Expression 1:** `!(A == B)`
<br>
**Expression 2:** `A != B`

These two expressions are the same. Here is the truth table:

| A | B | A == B | `!(A == B)` | `A != B `|
|---|---|--------|------------|---------| 
| 0 | 0 | 1 | 0 | 0 |
| 0 | 1 | 0 | 1 | 1 |
| 1 | 0 | 0 | 1 | 1 |
| 1 | 1 | 1 | 0 | 0 |

**Expression 1:** `!((A == B) || (A == C))`
<br>
**Expression 2:** `(A != B) && (A != C)`

These two expressions are the same. Here is the truth table:

| A | B | C | A == B | A == C | (A == B) \|\| (A == C) | `!((A == B) \|\| (A == C))` | `(A != B) && (A != C)` |
|---|---|---|--------|---------|------------------------|--------------------------|----------------------| 
| 0 | 0 | 0 | 1 | 1 | 1 | 0 | 0 |
| 0 | 0 | 1 | 1 | 0 | 1 | 0 | 0 |
| 0 | 1 | 0 | 0 | 1 | 1 | 0 | 0 |
| 0 | 1 | 1 | 0 | 0 | 0 | 1 | 1 |
| 1 | 0 | 0 | 0 | 1 | 1 | 0 | 0 |
| 1 | 0 | 1 | 0 | 0 | 0 | 1 | 1 |
| 1 | 1 | 0 | 1 | 0 | 1 | 0 | 0 |
| 1 | 1 | 1 | 1 | 1 | 1 | 0 | 0 |

**Expression 1:** `!((A == B) && (C > D))`
<br>
**Expression 2:** `(A != B) || (C <= D)`

These two expressions are the same. Here is the truth table:

| A | B | C | D | A == B | C > D | (A == B) && (C > D) | `!((A == B) && (C > D))` | `(A != B) \|\| (C <= D)` |
|---|---|---|---|--------|--------|-------------------|------------------------|--------------------| 
| 0 | 0 | 0 | 0 | 1 | 0 | 0 | 1 | 1 |
| 0 | 0 | 0 | 1 | 1 | 0 | 0 | 1 | 1 |
| 0 | 0 | 1 | 0 | 1 | 1 | 0 | 1 | 1 |
| 0 | 0 | 1 | 1 | 1 | 0 | 0 | 1 | 1 |
| 0 | 1 | 0 | 0 | 0 | 0 | 0 | 1 | 1 |
| 0 | 1 | 0 | 1 | 0 | 0 | 0 | 1 | 1 |
| 0 | 1 | 1 | 0 | 0 | 1 | 0 | 1 | 1 |
| 0 | 1 | 1 | 1 | 0 | 0 | 0 | 1 | 1 |
| 1 | 0 | 0 | 0 | 0 | 0 | 0 | 1 | 1 |
| 1 | 0 | 0 | 1 | 0 | 0 | 0 | 1 | 1 |
| 1 | 0 | 1 | 0 | 0 | 1 | 0 | 1 | 1 |
| 1 | 0 | 1 | 1 | 0 | 0 | 0 | 1 | 1 |
| 1 | 1 | 0 | 0 | 1 | 0 | 0 | 1 | 1 |
| 1 | 1 | 0 | 1 | 1 | 0 | 0 | 1 | 1 |
| 1 | 1 | 1 | 0 | 1 | 1 | 1 | 0 | 0 |
| 1 | 1 | 1 | 1 | 1 | 0 | 0 | 1 | 1 |